examples/opaque/client_proofs.v
@@ -19,22 +19,25 @@ Notation iProp := (iProp Σ).
 Lemma wp_client_session (uid pw : term) (c : val):
 {{{ cryptis_ctx
       ∗ hash_pred (opN.@"A_u") (λ _,  True)
+      ∗ hash_pred (opN.@"SK") (λ _,  False)
+      ∗ hash_pred (opN.@"K") (λ _,  False)
+      ∗ hash_pred (opN.@"α") (λ _,  True)
       ∗ channel c
       ∗ public uid
       ∗ minted uid
       ∗ minted pw }}}
 Client.session uid c pw
-{{{ x , RET x ; True }}}.
+{{{ x , RET (repr x) ; SK_priv x }}}.
 Proof.
-  iIntros "%ϕ [#Cryptis [#Hpred [#Hc [#pubuid [#minteduid #mintedpw]]]]] Hhl".
+  iIntros "%ϕ (#Cryptis & #HpredA_u & #HpredSK & #HpredK & #Hpredα & #Hc & #pubuid & #minteduid & #mintedpw) Hhl".
   wp_lam. wp_pures.
   wp_apply (wp_mk_nonce (fun _ => False)%I (fun _ => True)%I) => //.
   iIntros "%x_u %Hnoncex_u #Hmintedx_u #Hprivatex_u #Heqx_u #Hsx_uV #Heqx_uV Htokenx_u".
   wp_pures.
   wp_apply (wp_mk_nonce (fun _ => False)%I (fun _ => True)%I) => //.
   iIntros "%r %Hnoncer #Hmintedr #Hprivater #Heqr #HsrV #HeqrV Htokenr".
-  iAssert (public (TInv r) ↔ ▷ □ False)%I as "{HsrV} HsrV".
-  { admit. }
+  (* iAssert (public (TInv r) ↔ ▷ □ False)%I as "{HsrV} HsrV". *)
+  (* { admit. } *)
   wp_pures.
   wp_apply wp_H'.
   wp_apply wp_texp.
@@ -53,10 +56,7 @@ Proof.
   iApply exp_pred_intro1.
   by iApply "Heqr".
   iModIntro; iIntros "#p".
-  iApply False_public.
-  by rewrite minted_THash  minted_tag.
-  rewrite bi.intuitionistic_intuitionistically.
-  by iApply "HsrV".
+  iApply (public_THashIS with "Hpredα") => //.
   iApply public_TExp_iff; auto.
   do !iSplit => //.
   by iApply minted_TInt.
@@ -72,8 +72,8 @@ Proof.
   wp_list_of_term m2; wp_pures => //.
   wp_list_match => [β X_s envelope A_s -> | _].
   1, 2: wp_pures.
-  2, 3: by iApply "Hhl".
-  wp_apply wp_hl_inv_term.
+  2, 3: by iApply ("Hhl" $! None).
+wp_apply wp_hl_inv_term.
   wp_apply wp_texp.
   wp_list.
   wp_apply wp_H.
@@ -85,16 +85,16 @@ Proof.
   wp_apply wp_sdec'.
   rewrite minted_of_list => /=.
   iSplit.
-  2: iIntros "_"; wp_pures; by iApply "Hhl".
+  2: iIntros "_"; wp_pures; by iApply ("Hhl" $! None).
   iDestruct "minm2" as "[_ [minX_s [minenv _]]]".
   iIntros "%clear -> _".
   rewrite minted_TSeal.
   iDestruct "minenv" as "[mink minclear]".
   rewrite minted_tag.
   wp_list_of_term clear.
-  2: wp_pures; by iApply "Hhl".
+  2: wp_pures; by iApply ("Hhl" $! None).
   wp_list_match => [p_u P_u P_s -> | _].
-  2: wp_pures; by iApply "Hhl".
+  2: wp_pures; by iApply ("Hhl" $! None).
   wp_apply wp_ke => /=.
   wp_list.
   wp_apply wp_H => /=.
@@ -102,6 +102,8 @@ Proof.
   wp_apply wp_prf => /=.
   wp_list.
   wp_apply wp_prf.
+  rewrite minted_of_list => /=.
+  iDestruct "minclear" as "[minp_u [minP_u [minP_s _]]]".
   wp_eq_term eq_A_s => /= //.
   wp_list.
   wp_apply wp_prf.
@@ -109,7 +111,6 @@ Proof.
   wp_apply wp_send => //.
   iApply public_THashIS; eauto.
   rewrite !minted_of_list /=.
-  iDestruct "minclear" as "[minp_u [minP_u [minP_s _]]]".
   do !iSplit => //.
   rewrite minted_THash minted_tag minted_of_list.
   do !iSplit => //; iApply all_minted_TExp; iSplit => //.
@@ -119,10 +120,27 @@ Proof.
   iSplit => //.
   by rewrite minted_THash minted_tag.
   by intro contra.
-  2: wp_pures; by iApply "Hhl".
+  2: by wp_pures; iApply ("Hhl" $! None).
   wp_list.
   wp_pures.
-  by iApply "Hhl".
+  set SK := hash_result _ _.
+  iApply ("Hhl" $! (Some SK)).
+  iModIntro.
+  rewrite /SK_priv /SK.
+  iSplit; iIntros "contra".
+  iDestruct (public_THashE with "HpredSK contra") as "[contra | [_ contra]]" => //.
+  rewrite public_of_list.
+  iDestruct "contra" as "[contra _]".
+  iDestruct (public_THashE with "HpredK contra") as "[contra | [_ contra]]" => //.
+  rewrite public_of_list.
+  iDestruct "contra" as "(_ & contra & _)".
+  admit.
+  iApply (public_THashIS with "HpredSK") => //.
+  rewrite minted_of_list.
+  do !iSplit => //; rewrite minted_THash minted_tag minted_of_list; do !iSplit => //.
+  1, 2: rewrite -all_minted_TExp; iSplit => //.
+  rewrite -all_minted_TExp minted_THash minted_tag.
+  by iSplit => //.
 Admitted.
 
 End Opaque.
