examples/opaque/server_proofs.v
@@ -24,40 +24,31 @@ Notation iProp := (iProp Σ).
 Definition opaque_file (file : val) : iProp :=
   ∃ k_s p_s P_s P_u envelope,
     ⌜file = Spec.of_list [k_s; p_s; P_s; P_u; envelope]⌝
-    ∗ minted k_s ∗
+    ∗ minted k_s ∗ □(public k_s ↔ ▷ □ False) ∗
     □(∀ t' : term, exp_pred_base k_s t' ↔ ▷ □ True) ∗
     □(public (TInv k_s) ↔ ▷ False) ∗
     □(∀ t' : term, exp_pred_base (TInv k_s) t' ↔ ▷ False) ∗
-    minted p_s ∗ public P_s ∗ public P_u ∗ public envelope.
+    minted p_s ∗ □(public p_s ↔ ▷ □ False) ∗
+    □(∀ t' : term, exp_pred_base p_s t' ↔ ▷ □
+                                 ∃ (b: term) e,
+                                   ⌜TExp b e = t'⌝
+                                   ∗ match b with
+                                   | TInt _ => True
+                                   | _ => False
+                                   end) ∗
+    public P_s ∗ public P_u ∗ public envelope.
 
 Definition opaque_db (db : gmap term val) : iProp :=
 [∗ map] (k : term) ↦ (file : val) ∈ db,
 public k ∗ opaque_file file.
 
-Lemma public_THashE N φ t :
-  hash_pred N φ -∗
-  public (THash (Spec.tag (Tag N) t)) -∗
-  public t ∨ minted t ∗ ▷ □ φ t.
-Proof.
-  iIntros "#Hpred #Hpub".
-  rewrite public_THash.
-  iDestruct "Hpub" as "[Hpub | [Hmint Hwfhash]]".
-  rewrite public_tag.
-  by iLeft.
-  rewrite minted_tag.
-  iRight.
-  iSplit => //.
-  iDestruct (wf_hash_elim N t φ with "Hwfhash Hpred") as "H".
-  by iNext.
-Qed.
-
 Lemma wp_make_file (pw : term) (Φ : senc_key → term → iProp) :
 {{{ cryptis_ctx
-      ∗ minted pw
-      ∗ □ (public pw ↔ ▷ □ False)
-      ∗ hash_pred (opN.@"rw") (λ _,  False)
-      ∗ senc_pred (opN.@"AuthEnc") Φ
-      ∗ □ ∀ s t, Φ s t }}}
+    ∗ minted pw
+    ∗ □ (public pw ↔ ▷ □ False)
+    ∗ hash_pred (opN.@"rw") (λ _,  False)
+    ∗ senc_pred (opN.@"AuthEnc") Φ
+    ∗ □ ∀ s t, Φ s t }}}
 Server.make_file pw
 {{{ file , RET (repr file) ; opaque_file file }}}.
 Proof.
@@ -65,8 +56,8 @@ Proof.
   wp_lam.
   wp_apply (wp_mk_nonce (fun _ => False)%I (fun _ => True)%I) => //.
   iIntros "%k_s %Hnoncek_s #Hmintedk_s #Hprivatek_s #Heqk_s #Hsk_sV #Heqk_sV Htokenk_s".
-  iAssert (public (TInv k_s) ↔ ▷ False)%I as "{Hsk_sV} Hsk_sV".
-  { admit. }
+  (* iAssert (public (TInv k_s) ↔ ▷ False)%I as "{Hsk_sV} Hsk_sV". *)
+  (* { admit. } *)
   wp_pures.
   wp_lam.
   wp_pures.
@@ -76,8 +67,15 @@ Proof.
   wp_apply wp_H.
   wp_apply wp_derive_senc_key.
   wp_pures.
-  wp_apply (wp_mk_nonce (fun _ => False)%I (fun _ => True)%I) => //.
-  iIntros "%p_s %Hnoncep_s #Hmintedp_s #Hprivatep_s #Heqp_s #? #Heqp_sV Htokenp_s".
+  wp_apply (wp_mk_nonce (fun _ => False)%I
+                      (fun t => ∃ (b: term) e,
+                           ⌜TExp b e = t⌝
+                                         ∗ match b with
+                                           | TInt _ => True
+                                           | _ => False
+                                           end
+                      )%I) => //.
+  iIntros "%p_s %Hnoncep_s #Hmintedp_s #Hprivatep_s #Hexppredp_s #? #Hexppredp_sV Htokenp_s".
   wp_pures.
   wp_apply (wp_mk_nonce (fun _ => False)%I (fun _ => True)%I) => //.
   iIntros "%p_u %Hnoncep_u #Hmintedp_u #Hprivatep_u #Heqp_u #? #Heqp_uV Htokenp_u".
@@ -92,12 +90,15 @@ Proof.
   wp_term_of_list.
   iApply "post".
   iExists k_s, p_s, (TExp g p_s), (TExp g p_u), _.
-  do !iSplit => //.
+  do !iSplit => //.     
   1, 2: iApply public_TExp_iff; auto.
   1, 2: do !iSplit => //.
   1, 4: by iApply minted_TInt.
   iApply exp_pred_intro1.
-  by iApply "Heqp_s"; auto.
+  iApply "Hexppredp_s".
+  iNext. iModIntro.
+  iExists g, p_s.
+  by iSplit => //.
   1, 3: by rewrite public_TInt; auto.
   iApply exp_pred_intro1.
   by iApply "Heqp_u"; auto.
@@ -116,41 +117,44 @@ Proof.
   iDestruct "Hprivpw" as "[Hprivpw _]".
   iDestruct "Hpub" as "[Hpubpw _]".
   iDestruct ("Hprivpw" with "Hpubpw") as "contra".
-  all: iDestruct "Hprivatep_u" as "[_ Hprivatep_u]";
+  all: by iDestruct "Hprivatep_u" as "[_ Hprivatep_u]";
     iDestruct ("Hprivatep_u" with "contra") as "Hpubp_u";
     iDestruct "Hprivatep_s" as "[_ Hprivatep_s]";
     iDestruct ("Hprivatep_s" with "contra") as "Hpubp_s";
-    do !iSplit => //; do ?iApply public_TExp => //; by rewrite public_TInt.
-Admitted.
+    do !iSplit => //; do ?iApply public_TExp => //; rewrite public_TInt.
+Qed.
 
 Lemma wp_server_session (db c : val) (alist : gmap term val) :
 {{{ cryptis_ctx
-      ∗ hash_pred (opN.@"A_s") (λ _,  True)
-      ∗ channel c
-      ∗ AList.is_alist db alist
-      ∗ opaque_db alist }}}
-  Server.session db c
-{{{ x , RET x ; True }}}.
+    ∗ hash_pred (opN.@"A_s") (λ _,  True)
+    ∗ hash_pred (opN.@"SK") (λ _,  False)
+    ∗ hash_pred (opN.@"K") (λ _,  False)
+    ∗ channel c
+    ∗ AList.is_alist db alist
+    ∗ opaque_db alist }}}
+Server.session db c
+{{{ x , RET (repr x) ; SK_priv x }}}.
 Proof.
   iIntros "%ϕ".
   rewrite /opaque_db. rewrite big_sepM_forall.
-  iIntros "[#Cryptis [#Hpred [#Hc [Hdb #Hmapcontents]]]] Hhl".
+  iIntros "(#Cryptis & #HpredA_s & #HpredSK & #HpredK & #Hc & Hdb & #Hmapcontents) Hhl".
   wp_lam. wp_pures.
   wp_apply (wp_recv with "Hc").
   iIntros "%m1 #Hpubm1".
   wp_list_of_term m1; wp_pures.
-  2: by iApply "Hhl".
+  2: by iApply ("Hhl" $! None).
   do !rewrite subst_list_match /=.
   wp_list_match => [uid α X_u -> | _].
-  2: wp_pures; by iApply "Hhl".
+  2: by wp_pures; iApply ("Hhl" $! None).
   wp_bind (AList.find _ _).
   iApply (AList.wp_find with "Hdb").
   iIntros "!> Hdb".
   case db_uid: (alist !! uid) => [file|]; wp_pures.
-  2: by iApply "Hhl".
+  2: by iApply ("Hhl" $! None).
   iDestruct ("Hmapcontents" $! uid file with "[//]") as
   "[_ (%k_s & %p_s & %P_s & %P_u & %envelope &
-        %e & Hmk_s & Hexppredk_s & #? & Hmp_s & Hmp_sV & HpP_s & HpP_u & Hpenvelope)]".
+        %e & Hmk_s & Hprivk_s & Hexppredk_s & Hexppredk_sV &
+        Hmp_s & Hprivp_s & Hexpp_s & HpP_s & HpP_u & Hpenvelope)]".
   rewrite !subst_list_match /= e.
   wp_apply wp_list_of_term.
   rewrite Spec.of_listK.
@@ -199,10 +203,27 @@ Proof.
   wp_list.
   wp_apply wp_prf.
   wp_eq_term Heq; wp_pures.
-  2: by iApply "Hhl".
-  wp_list.
-  wp_pures.
-  by iApply "Hhl".
-Qed.
+  2: by iApply ("Hhl" $! None).
+  iModIntro.
+  set SK := hash_result _ _.
+  iApply ("Hhl" $! (Some SK)).
+  rewrite /SK_priv /SK.
+  iSplit => //.
+  iIntros "Hcontra".
+  iDestruct (public_THashE with "HpredSK Hcontra") as "[Hpub | [_ contra]]" => //.
+  rewrite public_of_list.
+  iDestruct "Hpub" as "[Hpub _]".
+  iDestruct (public_THashE with "HpredK Hpub") as "[Hpub | [_ contra]]" => //.
+  rewrite public_of_list.
+  iDestruct "Hpub" as "(_ & Hcontra & _)".
+  (* g^ab <-> false*)
+  admit.
+  iIntros "#contra".
+  iApply (public_THashIS with "HpredSK") => //.
+  rewrite minted_of_list.
+  do !iSplit => //; rewrite minted_THash minted_tag minted_of_list; do !iSplit => //.
+  1, 2: rewrite -all_minted_TExp; iSplit => //.
+  all: by iApply public_minted.
+Admitted.
 
 End Opaque.
